Partial extraction succeeds

qtesla/code/Hacl.Impl.QTesla.fst
@@ -36,7 +36,7 @@ module FS   = Spec.SHA3
 module SHA3 = Hacl.SHA3
 module S    = Spec.QTesla
 
-module R    = Hacl.Frodo.Random
+module R    = Hacl.QTesla.Random
 
 type poly = lbuffer elem (v params_n)
 type poly_k = lbuffer elem (v (params_k *. params_n))
@@ -54,7 +54,7 @@ val index_poly: p: poly_k -> k: size_t{k <. params_k} -> Stack poly
     (ensures fun h0 pk h1 -> h0 == h1 /\ pk == get_poly p k)
 let index_poly p k = sub p (k *. params_n) params_n
 
-let randomness_extended_size = (params_k +. (size 3)) *. crypto_seedbytes
+let randomness_extended_size = normalize_term ((params_k +. size 3) *. crypto_seedbytes)
 
 assume val cshake128_frodo:
     input_len:size_t
@@ -63,10 +63,10 @@ assume val cshake128_frodo:
   -> output_len:size_t
   -> output: lbuffer uint8 (v output_len)
   -> Stack unit
-    (requires fun h -> B.live h input /\ B.live h output /\ B.disjoint input output)
-    (ensures fun h0 _ h1 -> 
-      modifies (loc_buffer output) h0 h1 /\
-      B.as_seq h1 output == FS.cshake128_frodo (v input_len) (B.as_seq h0 input) cstm (v output_len))
+    (requires fun h -> live h input /\ live h output /\ disjoint input output)
+    (ensures fun h0 _ h1 ->
+      modifies1 output h0 h1 /\
+      as_seq h1 output == FS.cshake128_frodo (v input_len) (as_seq h0 input) cstm (v output_len))
 
 val cdtIndex:
     x : size_t
@@ -76,7 +76,7 @@ val cdtIndex:
 // TODO: Will need for implementation of sample_gauss_poly
 (*let cdtIndex x y = x *. (size 3) + y*)
 
-assume val sample_gauss_poly: 
+assume val sample_gauss_poly:
     x: poly
   -> seed: lbuffer uint8 (v crypto_randombytes)
   -> nonce: FStar.Int64.t
@@ -84,13 +84,13 @@ assume val sample_gauss_poly:
     (requires fun h -> live h x /\ live h seed /\ disjoint x seed)
     (ensures fun h0 _ h1 ->
       live h1 x /\ live h1 seed /\
-      modifies (loc_buffer x) h0 h1) // TODO: output equal to spec
+      modifies1 x h0 h1) // TODO: output equal to spec
 
 // TODO: There is all kinds of specialized per-parameter-set stuff happening in sample_gauss_poly.
 // Need to figure out how to write a more general parameterized implementation, or if it's necessary,
 // write a separate one for each parameter set.
 (*let sample_gauss_poly x seed nonce =
-    [@inline_let] 
+    [@inline_let]
     let cdtList: list I64.t = [
     0x0000020000000000L; 0x0000000000000000L; 0x0000000000000000L;
     0x0000030000000000L; 0x0000000000000000L; 0x0000000000000000L;
@@ -113,7 +113,7 @@ assume val sample_gauss_poly:
     let j = create #I64.t #1 (size 1) 0L in
     let bitsremained = create #I64.t #1 (size 1) 0L in
     let rbits = create #I64.t #1 (size 1) 0L in
-    let y = create #I64.t #1 
+    let y = create #I64.t #1
     let r = create #UI64.t #1 (size 1) 0uL in
     let s = create #UI64.t #1 (size 1) 0uL in
     let t = create #UI64.t #1 (size 1) 0uL in
@@ -125,51 +125,49 @@ assume val sample_gauss_poly:
 
     for 0ul params_n
         (fun h _ -> live h seed_ex /\ live h j)
-	(fun x_ind ->
-	    if let jVal = j.size(0) in jVal +. 46 >. params_n
-	    then ( params_gaussSampler_xof crypto_randombytes seed dmsp.(size 0) (params_n *. (size 8)) buf;
-	           j.(size 0) <- (size 0)
-		 )
+        (fun x_ind ->
+            if let jVal = j.size(0) in jVal +. 46 >. params_n
+            then ( params_gaussSampler_xof crypto_randombytes seed dmsp.(size 0) (params_n *. (size 8)) buf;
+                   j.(size 0) <- (size 0)
+                 )
             else ();
 
-            do_while 
-	        (fun h _ -> live h seed_ex /\ live h buf /\ live h j)
-		(fun _ ->
-		    rbits.(size 0) <- buf.(j.(size 0));
-		    j.(size 0) <- j.(size 0) +. (size 1);
+            do_while
+                (fun h _ -> live h seed_ex /\ live h buf /\ live h j)
+                (fun _ ->
+                    rbits.(size 0) <- buf.(j.(size 0));
+                    j.(size 0) <- j.(size 0) +. (size 1);
                     bitsremained.(size 0) <- 64L;
 
                     do_while
-		        (fun h -> live h seed_ex /\ live h buf /\ live h j)
-			(fun _ ->
-			    r.(size 0) <- buf.(j.(size 0));
-			    j.(size 0) <- I64.((j.(size 0)) +^ 1L);
-			    s.(size 0) <- buf.(j.(size 0));
-			    j.(size 0) <- I64.((j.(size 0)) +^ 1L);
-			    t.(size 0) <- buf.(j.(size 0));
-			    j.(size 0) <- I64.((j.(size 0)) +^ 1L);
+                        (fun h -> live h seed_ex /\ live h buf /\ live h j)
+                        (fun _ ->
+                            r.(size 0) <- buf.(j.(size 0));
+                            j.(size 0) <- I64.((j.(size 0)) +^ 1L);
+                            s.(size 0) <- buf.(j.(size 0));
+                            j.(size 0) <- I64.((j.(size 0)) +^ 1L);
+                            t.(size 0) <- buf.(j.(size 0));
+                            j.(size 0) <- I64.((j.(size 0)) +^ 1L);
                             if (let bitsremainedVal = bitsremainedVal.(size 0) in bitsremainedVal <=^ 64L - 6L)
-			    then rbits.(size 0) <- I64.t(((rbits.(size 0)) <<^ 6L) ^^ (((r.(size 0)) >>^ 58L) &^ 63L))
-			    else ();
-			    r.(size 0) <- I64.t(r.(size 0) &^ 0x000003FFFFFFFFFFL);
+                            then rbits.(size 0) <- I64.t(((rbits.(size 0)) <<^ 6L) ^^ (((r.(size 0)) >>^ 58L) &^ 63L))
+                            else ();
+                            r.(size 0) <- I64.t(r.(size 0) &^ 0x000003FFFFFFFFFFL);
 
                             I64.t(r.(size 0) >^ 0x0000032102010020L)
-			);
+                        );
 
                     y.(size 0) <- 0L;*)
-			    
+
 
 val sampleE_state: i:size_nat -> Type0
 let sampleE_state i = tuple2 S.polys_t S.positive
 
 // TODO: Better way of doing negation/absolute value of an Int64?
-val abs: 
-    x: elem
-  -> Tot elem
-let abs x = if x <^ (to_elem 0) then x *^ (to_elem (-1)) else x
+val abs_elem: elem -> elem
+let abs_elem x = if x <^ (to_elem 0) then x *^ (to_elem (-1)) else x
 
-val check_ES: 
-    p: poly 
+val check_ES:
+    p: poly
   -> bound: UI32.t
   -> Stack bool
     (requires fun h -> live h p)
@@ -177,35 +175,35 @@ val check_ES:
 
 let check_ES p bound =
   push_frame();
-  let sum = create #FStar.UInt32.t #1 (size 1) 0ul in
-  let limit = create #FStar.UInt32.t #1 (size 1) params_n in
-  let temp = create #FStar.Int16.t #1 (size 1) 0s in
-  let mask = create #FStar.Int16.t #1 (size 1) 0s in
-  let list = create #FStar.Int16.t #(v params_n) params_n 0s in
-  C.Loops.for (size 0) params_n
+  let sum = create (size 1) 0ul in
+  let limit = create (size 1) params_n in
+  let temp = create (size 1) 0s in
+  let mask = create (size 1) 0s in
+  let list = create params_n 0s in
+  for (size 0) params_n
       (fun h _ -> live h p /\ live h list)
       (fun j ->
-	let abspj:elem = abs p.(j) in
-	list.(j) <- elem_to_int16 abspj);
+        let abspj = abs_elem p.(j) in
+        list.(j) <- elem_to_int16 abspj);
 
-  C.Loops.for (size 0) params_h
+  for (size 0) params_h
       (fun h _ -> live h p /\ live h sum /\ live h limit /\ live h temp /\ live h mask /\ live h list)
       (fun j ->
           let loopMax:UI32.t = UI32.((limit.(0ul)) -^ 1ul) in
-          C.Loops.for 0ul loopMax
-	  (fun h _ -> live h p /\ live h sum /\ live h limit /\ live h temp /\ live h mask /\ live h list)
-	  (fun i32 ->
-	      let i = uint32_to_int16 i32 in
-	      mask.(size 0) <- I16.( (list.(i +^ 1s)) -^ (list.(i)) >>^ 15ul );
-	      temp.(size 0) <- I16.(( (list.(i +^ 1s)) &^ (mask.(0ul)) ) |^
-	                      ( (list.(i)) &^ (lognot mask.(size 0)) ));
-	      list.(I16.(i +^ 1s)) <- I16.(( (list.(i)) &^ mask.(0ul) ) |^
-	                                 ( (list.(i +^ 1s)) &^ (lognot mask.(0ul)) ));
+          for 0ul loopMax
+          (fun h _ -> live h p /\ live h sum /\ live h limit /\ live h temp /\ live h mask /\ live h list)
+          (fun i32 ->
+              let i = uint32_to_int16 i32 in
+              mask.(size 0) <- I16.( (list.(i +^ 1s)) -^ (list.(i)) >>^ 15ul );
+              temp.(size 0) <- I16.(( (list.(i +^ 1s)) &^ (mask.(0ul)) ) |^
+                              ( (list.(i)) &^ (lognot mask.(size 0)) ));
+              list.(I16.(i +^ 1s)) <- I16.(( (list.(i)) &^ mask.(0ul) ) |^
+                                         ( (list.(i +^ 1s)) &^ (lognot mask.(0ul)) ));
               list.(i) <- temp.(size 0)
-	  );
+          );
 
           let listIndex:UI32.t = UI32.((limit.(0ul)) -^ 1ul) in
-	  let listAmt:I16.t = list.(listIndex) in
+          let listAmt:I16.t = list.(listIndex) in
           let listAmt:UI32.t = int16_to_uint32 listAmt in
           sum.(size 0) <- UI32.(sum.(size 0) +^ listAmt);
           limit.(size 0) <- UI32.((limit.(size 0)) -^ 1ul)
@@ -244,74 +242,78 @@ val poly_uniform:
   -> seed: lbuffer uint8 (v crypto_randombytes)
   -> Stack unit
     (requires fun h -> live h a /\ live h seed /\ disjoint a seed)
-    (ensures fun h0 _ h1 -> live h1 a /\ live h1 seed /\ modifies (loc_buffer a) h0 h1)
+    (ensures fun h0 _ h1 -> live h1 a /\ live h1 seed /\ modifies1 a h0 h1)
 
 let poly_uniform a seed =
     push_frame();
-    let pos = create #size_t #1 (size 1) (u32 0) in
-    let i = create #size_t #1 (size 1) (u32 0) in
+    let pos = create (size 1) (size 0) in
+    let i = create (size 1) (u32 0) in
     let nbytes:size_t = (params_q_log +. 7ul) /. 8ul in
-    let nblocks = create #size_t #1 (size 1) params_genA in
+    let nblocks = create (size 1) params_genA in
     let mask:UI32.t = (1ul <<. params_q_log) -. 1ul in
-    let bufSize:size_t = (nblocks.(0ul)) *. shake128_rate in
-    let buf = create #uint8 #(v bufSize) bufSize (u8 0) in
-    let dmsp = create #UI16.t #1 (size 1) 0us in
+    let bufSize:size_t = nblocks.(0ul) *. shake128_rate in
+    let buf = create bufSize (u8 0) in
+    let dmsp = create (size 1) 0us in
     cshake128_frodo crypto_randombytes seed (dmsp.(0ul)) bufSize buf;
     dmsp.(0ul) <- UI16.((dmsp.(0ul)) +^ 1us);
 
-    C.Loops.while 
+    while
         #(fun h -> live h pos /\ live h i /\ live h nblocks /\ live h buf /\ live h dmsp)
-	#(fun _ h -> live h pos /\ live h i /\ live h nblocks /\ live h buf /\ live h dmsp)
+        #(fun _ h -> live h pos /\ live h i /\ live h nblocks /\ live h buf /\ live h dmsp)
         ( fun _ -> (i.(0ul)) <. (params_k *. params_n) )
-	( fun _ -> 
-	    let bufSize:size_t = (nblocks.(0ul)) *. shake128_rate in
-	    if (pos.(0ul)) >. bufSize -. (4ul *. nbytes)
-	    then ( nblocks.(0ul) <- 1ul;
-   	         let bufSize:size_t = (nblocks.(0ul)) *. shake128_rate in
-	         cshake128_frodo crypto_randombytes seed (dmsp.(0ul)) bufSize buf;
-		 dmsp.(0ul) <- UI16.((dmsp.(0ul)) +^ 1us);
-		 pos.(0ul) <- 0ul )
-	    else ();
+        ( fun _ ->
+            let bufSize:size_t = (nblocks.(0ul)) *. shake128_rate in
+            if (pos.(0ul)) >. bufSize -. (4ul *. nbytes)
+            then ( nblocks.(0ul) <- 1ul;
+                 let bufSize:size_t = (nblocks.(0ul)) *. shake128_rate in
+                 cshake128_frodo crypto_randombytes seed (dmsp.(0ul)) bufSize buf;
+                 dmsp.(0ul) <- UI16.((dmsp.(0ul)) +^ 1us);
+                 pos.(0ul) <- 0ul )
+            else ();
 
-	    let bufSize:size_t = (nblocks.(0ul)) *. shake128_rate in
+            let bufSize:size_t = (nblocks.(0ul)) *. shake128_rate in
 
-	    let subbuff = sub #_ #(v bufSize) #(numbytes U32) buf pos (size (numbytes U32)) in
-	    let bufPosAsUint = uint_from_bytes_le #U32 #PUB subbuff in
+            let pos0 = pos.(0ul) in
+            let subbuff = sub buf pos0 (size (numbytes U32)) in
+            let bufPosAsUint = uint_from_bytes_le #U32 #PUB subbuff in
             let val1 = bufPosAsUint &. mask in
-	    pos.(0ul) <- UI32.((pos.(0ul)) +^ nbytes);
+            pos.(0ul) <- UI32.(pos0 +^ nbytes);
 
-	    let subbuff = sub #_ #(v bufSize) #(numbytes U32) buf pos (size (numbytes U32)) in
-	    let bufPosAsUint = uint_from_bytes_le #U32 #PUB subbuff in
+            let pos0 = pos.(0ul) in
+            let subbuff = sub buf pos0 (size (numbytes U32)) in
+            let bufPosAsUint = uint_from_bytes_le #U32 #PUB subbuff in
             let val2 = bufPosAsUint &. mask in
-	    pos.(0ul) <- UI32.((pos.(0ul)) +^ nbytes);
-
-	    let subbuff = sub #_ #(v bufSize) #(numbytes U32) buf pos (size (numbytes U32)) in
-	    let bufPosAsUint = uint_from_bytes_le #U32 #PUB subbuff in
+            pos.(0ul) <- UI32.(pos0 +^ nbytes);
+            
+            let pos0 = pos.(0ul) in
+            let subbuff = sub buf pos0 (size (numbytes U32)) in
+            let bufPosAsUint = uint_from_bytes_le #U32 #PUB subbuff in
             let val3 = bufPosAsUint &. mask in
-	    pos.(0ul) <- UI32.((pos.(0ul)) +^ nbytes);
+            pos.(0ul) <- UI32.(pos0 +^ nbytes);
 
-	    let subbuff = sub #_ #(v bufSize) #(numbytes U32) buf pos (size (numbytes U32)) in
-	    let bufPosAsUint = uint_from_bytes_le #U32 #PUB subbuff in
+            let pos0 = pos.(0ul) in
+            let subbuff = sub buf pos0 (size (numbytes U32)) in
+            let bufPosAsUint = uint_from_bytes_le #U32 #PUB subbuff in
             let val4 = bufPosAsUint &. mask in
-	    pos.(0ul) <- UI32.((pos.(0ul)) +^ nbytes);
+            pos.(0ul) <- UI32.(pos0 +^ nbytes);
 
-	    if (let iVal = i.(0ul) in val1 <. params_q && iVal <. (params_k *. params_n))
-	    then ( a.(i.(0ul)) <- reduce I64.((uint32_to_int64 val1) *^ params_r2_invn); 
-	         i.(0ul) <- UI32.((i.(0ul)) +^ 1ul) )
-	    else ();
-	    if (let iVal = i.(0ul) in val2 <. params_q && iVal <. (params_k *. params_n))
-	    then ( a.(i.(0ul)) <- reduce I64.((uint32_to_int64 val2) *^ params_r2_invn); 
-	         i.(0ul) <- UI32.((i.(0ul)) +^ 1ul) )
-	    else ();
-	    if (let iVal = i.(0ul) in val3 <. params_q && iVal <. (params_k *. params_n))
-	    then ( a.(i.(0ul)) <- reduce I64.((uint32_to_int64 val3) *^ params_r2_invn); 
-	         i.(0ul) <- UI32.((i.(0ul)) +^ 1ul) )
-	    else ();
-	    if (let iVal = i.(0ul) in val4 <. params_q && iVal <. (params_k *. params_n))
-	    then ( a.(i.(0ul)) <- reduce I64.((uint32_to_int64 val4) *^ params_r2_invn); 
-	         i.(0ul) <- UI32.((i.(0ul)) +^ 1ul) )
-	    else ()
-	);
+            if (let iVal = i.(0ul) in val1 <. params_q && iVal <. (params_k *. params_n))
+            then ( a.(i.(0ul)) <- reduce I64.((uint32_to_int64 val1) *^ params_r2_invn);
+                 i.(0ul) <- UI32.((i.(0ul)) +^ 1ul) )
+            else ();
+            if (let iVal = i.(0ul) in val2 <. params_q && iVal <. (params_k *. params_n))
+            then ( a.(i.(0ul)) <- reduce I64.((uint32_to_int64 val2) *^ params_r2_invn);
+                 i.(0ul) <- UI32.((i.(0ul)) +^ 1ul) )
+            else ();
+            if (let iVal = i.(0ul) in val3 <. params_q && iVal <. (params_k *. params_n))
+            then ( a.(i.(0ul)) <- reduce I64.((uint32_to_int64 val3) *^ params_r2_invn);
+                 i.(0ul) <- UI32.((i.(0ul)) +^ 1ul) )
+            else ();
+            if (let iVal = i.(0ul) in val4 <. params_q && iVal <. (params_k *. params_n))
+            then ( a.(i.(0ul)) <- reduce I64.((uint32_to_int64 val4) *^ params_r2_invn);
+                 i.(0ul) <- UI32.((i.(0ul)) +^ 1ul) )
+            else ()
+        );
 
     pop_frame()
 
@@ -323,52 +325,56 @@ val ntt:
   -> w: poly
   -> Stack unit
     (requires fun h -> live h a /\ live h w)
-    (ensures fun h0 _ h1 -> live h1 a /\ live h1 w /\ modifies (loc_buffer a) h0 h1)
+    (ensures fun h0 _ h1 -> live h1 a /\ live h1 w /\ modifies1 a h0 h1)
 
 let ntt a w =
     push_frame();
-    let numoProblems = create #size_t #1 (size 1) (params_n >>. (size 1)) in
-    let jTwiddle = create #size_t #1 (size 1) (size 0) in
+    let numoProblems = create (size 1) (params_n >>. (size 1)) in
+    let jTwiddle = create (size 1) (size 0) in
 
-    C.Loops.while // Outermost for loop
+    while // Outermost for loop
         #(fun h -> live h numoProblems /\ live h jTwiddle)
-	#(fun _ h -> live h numoProblems /\ live h jTwiddle)
+        #(fun _ h -> live h numoProblems /\ live h jTwiddle)
         (fun _ -> numoProblems.(size 0) >. (size 0))
-	(fun _ -> 
-	    push_frame();
-	    let j = create #size_t #1 (size 1) (size 0) in
-	    let jFirst = create #size_t #1 (size 1) (size 0) in
-	    C.Loops.while // Middle for loop
-	        #(fun h -> live h numoProblems /\ live h jTwiddle /\ live h j /\ live h jFirst)
-		#(fun _ h -> live h numoProblems /\ live h jTwiddle /\ live h j /\ live h jFirst)
-	        (fun _ -> jFirst.(size 0) <. params_n)
-		(fun _ ->
-	            let jTwiddleVal = jTwiddle.(size 0) in
-	            let wj:elem = w.(jTwiddleVal) in
-	            jTwiddle.(size 0) <- jTwiddleVal +. (size 1);
-		    // Innermost for loop. Have to use a while because the middle for loop's increment depends on the
-		    // final value of j from each inner for loop, so its scope can't be constrained to the for loop.
-		    j.(size 0) <- jFirst.(size 0);
-    		    let jFinish:UI32.t = UI32.(jFirst.(size 0) +^ numoProblems.(size 0)) in
-		    C.Loops.while
-		        #(fun h -> live h numoProblems /\ live h jTwiddle /\ live h jFirst)
-			#(fun _ h -> live h numoProblems /\ live h jTwiddle /\ live h jFirst)
-			(fun _ -> j.(size 0) <. jFinish)
-			(fun _ ->
-			    let jVal:size_t = j.(size 0) in
-			    let aIndex:size_t = UI32.(jVal +^ numoProblems.(size 0)) in
-			    let aVal:elem = a.(aIndex) in
-		            let temp:elem = barr_reduce (reduce I64.((elem_to_int64 wj) *^ (elem_to_int64 aVal))) in
-			    let aVal:elem = a.(jVal) in
-			    a.(aIndex) <- barr_reduce (int64_to_elem I64.((elem_to_int64 aVal) +^ (2L *^ (elem_to_int64 params_q) -^ (elem_to_int64 temp))));
-			    a.(j) <- barr_reduce (int64_to_elem I64.((elem_to_int64 temp) +^ ((elem_to_int64 aVal))))
-		        );
-		    jFirst.(size 0) <- UI32.(j.(size 0) +^ numoProblems.(size 0))
-		);
-	    numoProblems.(size 0) <- UI32.(numoProblems.(size 0) >>^ 1ul);
-	    pop_frame()
-	);
-
+        (fun _ ->
+            push_frame();
+            let j = create (size 1) (size 0) in
+            let jFirst = create (size 1) (size 0) in            
+            let cond () : Stack bool
+              (requires fun h -> live h jFirst)
+              (ensures fun h0 _ h1 -> live h1 jFirst)
+            = true in //jFirst.(size 0) <. params_n in
+            while // Middle for loop
+                #(fun h -> live h numoProblems /\ live h jTwiddle /\ live h j /\ live h jFirst)
+                #(fun _ h -> live h numoProblems /\ live h jTwiddle /\ live h j /\ live h jFirst)
+                cond
+                (fun _ -> ());
+                (*
+                    let jTwiddleVal = jTwiddle.(size 0) in
+                    let wj:elem = w.(jTwiddleVal) in
+                    jTwiddle.(size 0) <- jTwiddleVal +. (size 1);
+                    // Innermost for loop. Have to use a while because the middle for loop's increment depends on the
+                    // final value of j from each inner for loop, so its scope can't be constrained to the for loop.
+                    j.(size 0) <- jFirst.(size 0);
+                    let jFinish:UI32.t = UI32.(jFirst.(size 0) +^ numoProblems.(size 0)) in
+                    while
+                        #(fun h -> live h numoProblems /\ live h jTwiddle /\ live h jFirst)
+                        #(fun _ h -> live h numoProblems /\ live h jTwiddle /\ live h jFirst)
+                        (fun _ -> j.(size 0) <. jFinish)
+                        (fun _ ->
+                            let jVal:size_t = j.(size 0) in
+                            let aIndex:size_t = UI32.(jVal +^ numoProblems.(size 0)) in
+                            let aVal:elem = a.(aIndex) in
+                            let temp:elem = barr_reduce (reduce I64.((elem_to_int64 wj) *^ (elem_to_int64 aVal))) in
+                            let aVal:elem = a.(jVal) in
+                            a.(aIndex) <- barr_reduce (int64_to_elem I64.((elem_to_int64 aVal) +^ (2L *^ (elem_to_int64 params_q) -^ (elem_to_int64 temp))));
+                            a.(j) <- barr_reduce (int64_to_elem I64.((elem_to_int64 temp) +^ ((elem_to_int64 aVal))))
+                        );
+                    jFirst.(size 0) <- UI32.(j.(size 0) +^ numoProblems.(size 0))
+                );*)
+            numoProblems.(size 0) <- UI32.(numoProblems.(size 0) >>^ 1ul);
+            pop_frame()
+        );
     pop_frame()
 
 val nttinv:
@@ -376,50 +382,54 @@ val nttinv:
   -> w: poly
   -> Stack unit
     (requires fun h -> live h a /\ live h w)
-    (ensures fun h0 _ h1 -> live h1 a /\ live h1 w /\ modifies (loc_buffer a) h0 h1)
+    (ensures fun h0 _ h1 -> live h1 a /\ live h1 w /\ modifies1 a h0 h1)
 
-let nttinv a w = 
+let nttinv a w =
     push_frame();
-    let numoProblems = create #size_t #1 (size 1) (size 1) in
-    let jTwiddle = create #size_t #1 (size 1) (size 0) in
+    let numoProblems = create (size 1) (size 1) in
+    let jTwiddle = create (size 1) (size 0) in
 
     C.Loops.while // Outermost for loop
         #(fun h -> live h numoProblems /\ live h jTwiddle)
-	#(fun _ h -> live h numoProblems /\ live h jTwiddle)
+        #(fun _ h -> live h numoProblems /\ live h jTwiddle)
         (fun _ -> numoProblems.(size 0) >. (size 0))
-	(fun _ -> 
-	    push_frame();
-	    let j = create #size_t #1 (size 1) (size 0) in
-	    let jFirst = create #size_t #1 (size 1) (size 0) in
-	    C.Loops.while // Middle for loop
-	        #(fun h -> live h numoProblems /\ live h jTwiddle /\ live h j /\ live h jFirst)
-		#(fun _ h -> live h numoProblems /\ live h jTwiddle /\ live h j /\ live h jFirst)
-	        (fun _ -> jFirst.(size 0) <. params_n)
-		(fun _ ->
-	            let jTwiddleVal = jTwiddle.(size 0) in
-	            let wj:elem = w.(jTwiddleVal) in
-	            jTwiddle.(size 0) <- jTwiddleVal +. (size 1);
-		    // Innermost for loop. Have to use a while because the middle for loop's increment depends on the
-		    // final value of j from each inner for loop, so its scope can't be constrained to the for loop.
-		    j.(size 0) <- jFirst.(size 0);
-    		    let jFinish:UI32.t = UI32.(jFirst.(size 0) +^ numoProblems.(size 0)) in
-		    C.Loops.while
-		        #(fun h -> live h numoProblems /\ live h jTwiddle /\ live h jFirst)
-			#(fun _ h -> live h numoProblems /\ live h jTwiddle /\ live h jFirst)
-			(fun _ -> j.(size 0) <. jFinish)
-			(fun _ ->
-			    let jVal:size_t = j.(size 0) in
-			    let aIndex:size_t = UI32.(jVal +^ numoProblems.(size 0)) in
-		            let temp:elem = a.(j) in
-			    let aaIndex:elem = a.(aIndex) in
-			    a.(j) <- barr_reduce (int64_to_elem I64.((elem_to_int64 temp) +^ (elem_to_int64 aaIndex)));
-			    a.(aIndex) <- barr_reduce (reduce I64.((elem_to_int64 wj) *^ ((elem_to_int64 temp) +^ (2L *^ (elem_to_int64 params_q) -^ (elem_to_int64 aaIndex)))))
-		        );
-		    jFirst.(size 0) <- UI32.(j.(size 0) +^ numoProblems.(size 0))
-		);
-	    numoProblems.(size 0) <- UI32.(numoProblems.(size 0) *^ 2ul);
-	    pop_frame()
-	);
+        (fun _ ->
+            push_frame();
+            let j = create (size 1) (size 0) in
+            let jFirst = create (size 1) (size 0) in
+            let cond () : Stack bool
+              (requires fun h -> live h jFirst)
+              (ensures fun h0 _ h1 -> live h1 jFirst)
+            = true in //jFirst.(size 0) <. params_n in
+            C.Loops.while // Middle for loop
+                #(fun h -> live h numoProblems /\ live h jTwiddle /\ live h j /\ live h jFirst)
+                #(fun _ h -> live h numoProblems /\ live h jTwiddle /\ live h j /\ live h jFirst)
+                cond
+                (fun _ ->
+                    let jTwiddleVal = jTwiddle.(size 0) in
+                    let wj:elem = w.(jTwiddleVal) in
+                    jTwiddle.(size 0) <- jTwiddleVal +. (size 1);
+                    // Innermost for loop. Have to use a while because the middle for loop's increment depends on the
+                    // final value of j from each inner for loop, so its scope can't be constrained to the for loop.
+                    j.(size 0) <- jFirst.(size 0);
+                    let jFinish:UI32.t = UI32.(jFirst.(size 0) +^ numoProblems.(size 0)) in
+                    C.Loops.while
+                        #(fun h -> live h numoProblems /\ live h jTwiddle /\ live h jFirst)
+                        #(fun _ h -> live h numoProblems /\ live h jTwiddle /\ live h jFirst)
+                        (fun _ -> j.(size 0) <. jFinish)
+                        (fun _ ->
+                            let jVal:size_t = j.(size 0) in
+                            let aIndex:size_t = UI32.(jVal +^ numoProblems.(size 0)) in
+                            let temp:elem = a.(j) in
+                            let aaIndex:elem = a.(aIndex) in
+                            a.(j) <- barr_reduce (int64_to_elem I64.((elem_to_int64 temp) +^ (elem_to_int64 aaIndex)));
+                            a.(aIndex) <- barr_reduce (reduce I64.((elem_to_int64 wj) *^ ((elem_to_int64 temp) +^ (2L *^ (elem_to_int64 params_q) -^ (elem_to_int64 aaIndex)))))
+                        );
+                    jFirst.(size 0) <- UI32.(j.(size 0) +^ numoProblems.(size 0))
+                );
+            numoProblems.(size 0) <- UI32.(numoProblems.(size 0) *^ 2ul);
+            pop_frame()
+        );
 
     pop_frame()
 
@@ -428,7 +438,7 @@ val poly_ntt:
   -> x: poly
   -> Stack unit
     (requires fun h -> live h x_ntt /\ live h x /\ disjoint x_ntt x)
-    (ensures fun h0 _ h1 -> live h1 x_ntt /\ live h1 x /\ modifies (loc_buffer x) h0 h1)
+    (ensures fun h0 _ h1 -> live h1 x_ntt /\ live h1 x /\ modifies1 x h0 h1)
 
 let poly_ntt x_ntt x =
     push_frame();
@@ -447,7 +457,7 @@ val poly_pointwise:
   -> y: poly
   -> Stack unit
     (requires fun h -> live h result /\ live h x /\ live h y)
-    (ensures fun h0 _ h1 -> live h1 result /\ live h1 x /\ live h1 y /\ modifies (loc_buffer result) h0 h1)
+    (ensures fun h0 _ h1 -> live h1 result /\ live h1 x /\ live h1 y /\ modifies1 result h0 h1)
 
 let poly_pointwise result x y =
     push_frame();
@@ -455,7 +465,7 @@ let poly_pointwise result x y =
     (fun h _ -> live h result /\ live h x /\ live h y)
     (fun i ->
         let xi:elem = x.(i) in
-	let yi:elem = y.(i) in
+        let yi:elem = y.(i) in
         result.(i) <- reduce I64.( (elem_to_int64 xi) *^ (elem_to_int64 yi) )
     );
     pop_frame()
@@ -466,7 +476,7 @@ val poly_mul:
   -> y: poly
   -> Stack unit
     (requires fun h -> live h result /\ live h x /\ live h y)
-    (ensures fun h0 _ h1 -> live h1 result /\ live h1 x /\ live h1 y /\ modifies (loc_buffer result) h0 h1)
+    (ensures fun h0 _ h1 -> live h1 result /\ live h1 x /\ live h1 y /\ modifies1 result h0 h1)
 
 // TODO
 assume val zetainv: poly
@@ -474,7 +484,7 @@ assume val zetainv: poly
 let poly_mul result x y =
     poly_pointwise result x y;
     nttinv result zetainv;
-    ()  
+    ()
 
 val poly_add:
     result: poly
@@ -482,7 +492,7 @@ val poly_add:
   -> y: poly
   -> Stack unit
     (requires fun h -> live h result /\ live h x /\ live h y /\ disjoint result x /\ disjoint result y /\ disjoint x y)
-    (ensures fun h0 _ h1 -> live h1 result /\ live h1 x /\ live h1 y /\ modifies (loc_buffer result) h0 h1)
+    (ensures fun h0 _ h1 -> live h1 result /\ live h1 x /\ live h1 y /\ modifies1 result h0 h1)
 
 let poly_add result x y =
     push_frame();
@@ -499,7 +509,7 @@ val poly_sub:
   -> y: poly
   -> Stack unit
     (requires fun h -> live h result /\ live h x /\ live h y)
-    (ensures fun h0 _ h1 -> live h1 result /\ live h1 x /\ live h1 y /\ modifies (loc_buffer result) h0 h1)
+    (ensures fun h0 _ h1 -> live h1 result /\ live h1 x /\ live h1 y /\ modifies1 result h0 h1)
 
 let poly_sub result x y =
     push_frame();
@@ -507,7 +517,7 @@ let poly_sub result x y =
     (fun h _ -> live h result /\ live h x /\ live h y)
     (fun i ->
         let xi:elem = x.(i) in
-	let yi:elem = y.(i) in
+        let yi:elem = y.(i) in
         result.(i) <- barr_reduce (x.(i) -^ y.(i))
     );
     pop_frame()
@@ -522,8 +532,8 @@ assume val pack_sk:
   -> Stack unit
     (requires fun h -> live h sk /\ live h s /\ live h e /\ live h seeds /\
                     disjoint sk s /\ disjoint sk e /\ disjoint sk seeds /\
-		    disjoint s e /\ disjoint s seeds /\ disjoint e seeds)
-    (ensures fun h0 _ h1 -> modifies (loc_buffer sk) h0 h1)
+                    disjoint s e /\ disjoint s seeds /\ disjoint e seeds)
+    (ensures fun h0 _ h1 -> modifies1 sk h0 h1)
 
 (*let pack_sk sk s e seeds =
     push_frame();
@@ -541,8 +551,8 @@ assume val pack_sk:
     (fun h0 _ -> live h0 isk /\ live h0 e)
     (fun k -> for 0ul params_n
            (fun h1 _ -> live h1 isk /\ live h1 e)
-	   (fun i -> isk.(params_n +. k *. params_n +. i) <- let eVal = e.(k *. params_n +. i) in
- 	                                                     int64_to_int8 eVal)
+           (fun i -> isk.(params_n +. k *. params_n +. i) <- let eVal = e.(k *. params_n +. i) in
+                                                             int64_to_int8 eVal)
     );
 
     update_sub isk (params_n +. params_k *. params_n) ((size 2) *. crypto_seedbytes) seeds;
@@ -564,7 +574,7 @@ assume val encode_pk:
   -> Stack unit
     (requires fun h -> live h pk /\ live h t /\ live h seedA /\
                     disjoint pk t /\ disjoint pk seedA /\ disjoint t seedA)
-    (ensures fun h0 _ h1 -> modifies (loc_buffer pk) h0 h1)
+    (ensures fun h0 _ h1 -> modifies (loc pk) h0 h1)
 
 assume val decode_pk:
     pk: buffer uint8
@@ -572,7 +582,7 @@ assume val decode_pk:
   -> pk_in: buffer uint8
   -> Stack unit
     (requires fun h -> live h pk /\ live h seedA /\ live h pk_in /\ disjoint pk seedA /\ disjoint pk pk_in /\ disjoint seedA pk_in)
-    (ensures fun h0 _ h1 -> modifies (loc_buffer pk) h0 h1 /\ modifies (loc_buffer seedA) h0 h1)
+    (ensures fun h0 _ h1 -> modifies (loc pk |+| loc seedA) h0 h1)
 
 assume val encode_sig:
     sm: buffer uint8
@@ -580,7 +590,7 @@ assume val encode_sig:
   -> z: poly
   -> Stack unit
     (requires fun h -> live h sm /\ live h c /\ live h z /\ disjoint sm c /\ disjoint sm z /\ disjoint c z)
-    (ensures fun h0 _ h1 -> modifies (loc_buffer sm) h0 h1)
+    (ensures fun h0 _ h1 -> modifies (loc sm) h0 h1)
 
 assume val decode_sig:
     c: buffer uint8
@@ -588,7 +598,7 @@ assume val decode_sig:
   -> sm: buffer uint8
   -> Stack unit
     (requires fun h -> live h c /\ live h z /\ live h sm /\ disjoint c z /\ disjoint c sm /\ disjoint z sm)
-    (ensures fun h0 _ h1 -> modifies (loc_buffer z) h0 h1 /\ modifies (loc_buffer c) h0 h1) 
+    (ensures fun h0 _ h1 -> modifies (loc z |+| loc c) h0 h1)
 
 val qtesla_keygen:
     pk: buffer uint8
@@ -599,11 +609,11 @@ val qtesla_keygen:
     (ensures fun _ _ _ -> True)
 
 // Preliminary work using one of Santiago's loop combinators for the first for loop
-(*assume val keygen_sample_spec: 
-    #rlen:size_nat 
-  -> rand:Lib.ByteSequence.lbytes rlen 
-  -> nonce:nat 
-  -> i:size_nat 
+(*assume val keygen_sample_spec:
+    #rlen:size_nat
+  -> rand:Lib.ByteSequence.lbytes rlen
+  -> nonce:nat
+  -> i:size_nat
   -> e:LibSeq.lseq poly (v params_k)
   -> Tot (LibSeq.lseq poly (v params_k))*)
 //let keygen_sample_spec #rlen rand nonce i e ="*)
@@ -615,58 +625,58 @@ val qtesla_keygen:
     C.Loops.do_while
       (fun h break -> live h e /\ live h randomness_extended /\
                    (not break ==> (check_ES (get h e k) params_Le)) /\
-		   (break ==> (not (check_ES (get h e k) params_Le))))
+                   (break ==> (not (check_ES (get h e k) params_Le))))
       (fun _ ->
         let nonce0 = nonce.(size 0) in
-	nonce.(size 0) <- nonce0 +. 1;
-	sample_gauss_poly e.(k) (sub randomness_extended (k * crypto_seedbytes) crypto_randombytes) nonce;
-	not (check_ES e.(k) params_Le)));*)
+        nonce.(size 0) <- nonce0 +. 1;
+        sample_gauss_poly e.(k) (sub randomness_extended (k * crypto_seedbytes) crypto_randombytes) nonce;
+        not (check_ES e.(k) params_Le)));*)
 
 let qtesla_keygen pk sk =
   push_frame();
-  let randomness = create #_ #(v crypto_randombytes) crypto_randombytes (u8 0) in
-  let randomness_extended = create #_ #(v randomness_extended_size) randomness_extended_size (u8 0) in
-  let e:poly_k = create #_ #(v (params_n *. params_k)) (params_n *. params_k) (to_elem 0) in
-  let s:poly = create #_ #(v params_n) params_n (to_elem 0) in	    
-  let s_ntt:poly = create #_ #(v params_n) params_n (to_elem 0) in
-  let a:poly_k = create #_ #(v (params_n *. params_k)) (params_n *. params_k) (to_elem 0) in
-  let t:poly_k = create #_ #(v (params_n *. params_k)) (params_n *. params_k) (to_elem 0) in
+  let randomness = create crypto_randombytes (u8 0) in
+  let randomness_extended = create randomness_extended_size (u8 0) in
+  let e:poly_k = create (params_n *. params_k) (to_elem 0) in
+  let s:poly = create params_n (to_elem 0) in
+  let s_ntt:poly = create params_n (to_elem 0) in
+  let a:poly_k = create (params_n *. params_k) (to_elem 0) in
+  let t:poly_k = create (params_n *. params_k) (to_elem 0) in
   // TODO: nonce and mask are signed types! Investigate this.
-  let nonce = create #FStar.Int64.t #1 1ul 0L in
-  let mask = create #elem #1 1ul (to_elem 0) in  
+  let nonce = create 1ul 0L in
+  let mask = create 1ul (to_elem 0) in
   R.randombytes_ crypto_randombytes randomness;
   SHA3.shake128_hacl crypto_randombytes randomness randomness_extended_size randomness_extended;
- 
+
   C.Loops.for (size 0) params_k
       (fun h _ -> live h nonce /\ live h e /\ live h randomness_extended)
       (fun k ->
-	C.Loops.do_while 
-	  (fun h break -> live h nonce /\ live h e /\ live h randomness_extended)
-		       //(break ==> (not (check_ES (get_poly e k) params_Le))))
-	  (fun _ ->
-	    let subbuffer = sub #_ #(v randomness_extended_size) #(v crypto_randombytes) randomness_extended (k *. crypto_seedbytes) crypto_randombytes in
+        C.Loops.do_while
+          (fun h break -> live h nonce /\ live h e /\ live h randomness_extended)
+                       //(break ==> (not (check_ES (get_poly e k) params_Le))))
+          (fun _ ->
+            let subbuffer = sub randomness_extended (k *. crypto_seedbytes) crypto_randombytes in
             let nonce0 = nonce.(0ul) in
-	    nonce.(0ul) <- I64.(nonce0 +^ 1L);
-	    let nonce1:uint64 = nonce.(0ul) in
-	    let ek:poly = index_poly e k in
-	    sample_gauss_poly ek subbuffer nonce1;
-	    // TODO: ek is a buffer, and so we shouldn't have to refetch it with index_poly to operate on its current value, right?
-	    not (check_ES ek params_Le)
-	  )
+            nonce.(0ul) <- I64.(nonce0 +^ 1L);
+            let nonce1:uint64 = nonce.(0ul) in
+            let ek:poly = index_poly e k in
+            sample_gauss_poly ek subbuffer nonce1;
+            // TODO: ek is a buffer, and so we shouldn't have to refetch it with index_poly to operate on its current value, right?
+            not (check_ES ek params_Le)
+          )
       );
   C.Loops.do_while
-      (fun h break -> live h s /\ live h randomness_extended /\ live h nonce) 
-		   //(break ==> (not (check_ES s params_Ls)))) // TODO: need Ghost/Tot version of check_ES for invariants
+      (fun h break -> live h s /\ live h randomness_extended /\ live h nonce)
+                   //(break ==> (not (check_ES s params_Ls)))) // TODO: need Ghost/Tot version of check_ES for invariants
       (fun _ ->
-	let rndsubbuffer = sub #_ #(v randomness_extended_size) #(v crypto_randombytes) randomness_extended (params_k *. crypto_seedbytes) crypto_randombytes in
+        let rndsubbuffer = sub randomness_extended (params_k *. crypto_seedbytes) crypto_randombytes in
         let nonce0:uint64 = nonce.(size 0) in
-	nonce.(size 0) <- nonce0 +. (u64 1);
-	let nonce1:uint64 = nonce.(size 0) in
-	sample_gauss_poly s rndsubbuffer nonce1;
-	not (check_ES s params_Ls)
+        nonce.(size 0) <- nonce0 +. (u64 1);
+        let nonce1:uint64 = nonce.(size 0) in
+        sample_gauss_poly s rndsubbuffer nonce1;
+        not (check_ES s params_Ls)
       );
 
-  let rndsubbuffer = sub #_ #(v randomness_extended_size) #(v crypto_randombytes) randomness_extended ((params_k +. (size 1)) *. crypto_seedbytes) crypto_randombytes in
+  let rndsubbuffer = sub randomness_extended ((params_k +. (size 1)) *. crypto_seedbytes) crypto_randombytes in
   poly_uniform a rndsubbuffer;
   poly_ntt s_ntt s;
 
@@ -674,19 +684,19 @@ let qtesla_keygen pk sk =
       (fun h _ -> live h t /\ live h a /\ live h s_ntt /\ live h e /\ live h mask)
       (fun k ->
           let tk:poly = index_poly t k in
-	  let ak:poly = index_poly a k in
-	  let ek:poly = index_poly e k in
+          let ak:poly = index_poly a k in
+          let ek:poly = index_poly e k in
           poly_mul tk ak s_ntt;
-	  poly_add tk tk ek;
-	  C.Loops.for 0ul params_n
-	  (fun h _ -> live h t /\ live h a /\ live h s_ntt /\ live h e /\ live h mask)
-	  (fun i ->
-	      let tki:elem = tk.(i) in
+          poly_add tk tk ek;
+          C.Loops.for 0ul params_n
+          (fun h _ -> live h t /\ live h a /\ live h s_ntt /\ live h e /\ live h mask)
+          (fun i ->
+              let tki:elem = tk.(i) in
               mask.(0ul) <- (params_q -^ tki) >>^ 63ul;
-	      let mask0:elem = mask.(size 0) in
-	      tk.(i) <- tki -^ (params_q &^ mask0)
-	   )
-	);
+              let mask0:elem = mask.(size 0) in
+              tk.(i) <- tki -^ (params_q &^ mask0)
+           )
+        );
 
   pack_sk sk s e rndsubbuffer;
   encode_pk pk t rndsubbuffer;
@@ -707,7 +717,7 @@ assume val hash_vm:
   -> hm : buffer uint8
   -> Stack unit
     (requires fun h -> live h c_bin /\ live h v /\ live h hm /\ disjoint c_bin v /\ disjoint c_bin hm /\ disjoint v hm)
-    (ensures fun h0 _ h1 -> live h1 c_bin /\ live h1 v /\ live h1 hm /\ modifies (loc_buffer c_bin) h0 h1)
+    (ensures fun h0 _ h1 -> live h1 c_bin /\ live h1 v /\ live h1 hm /\ modifies (loc c_bin) h0 h1)
 
 assume val encode_c:
     pos_list : lbuffer UI32.t (v params_h)
@@ -716,8 +726,7 @@ assume val encode_c:
   -> Stack unit
     (requires fun h -> live h pos_list /\ live h sign_list /\ live h c_bin /\ disjoint pos_list sign_list /\
                     disjoint pos_list c_bin /\ disjoint sign_list c_bin)
-    (ensures fun h0 _ h1 -> live h1 pos_list /\ live h1 sign_list /\ live h1 c_bin /\ modifies (loc_buffer pos_list) h0 h1 /\
-                         modifies (loc_buffer sign_list) h0 h1)
+    (ensures fun h0 _ h1 -> live h1 pos_list /\ live h1 sign_list /\ live h1 c_bin /\ modifies2 pos_list sign_list h0 h1)
 
 assume val sparse_mul8:
     prod : poly
@@ -726,7 +735,7 @@ assume val sparse_mul8:
   -> sign_list : lbuffer I16.t (v params_h)
   -> Stack unit
     (requires fun h -> live h prod /\ live h sk /\ live h pos_list /\ live h sign_list /\ disjoint prod sk /\ disjoint prod pos_list /\ disjoint prod sign_list)
-    (ensures fun h0 _ h1 -> live h1 prod /\ live h1 sk /\ live h1 pos_list /\ live h1 sign_list /\ modifies (loc_buffer prod) h0 h1)
+    (ensures fun h0 _ h1 -> live h1 prod /\ live h1 sk /\ live h1 pos_list /\ live h1 sign_list /\ modifies1 prod h0 h1)
 
 assume val test_rejection:
     z : poly
@@ -748,28 +757,27 @@ val crypto_sign:
   -> mlen : size_t{B.length m = v mlen}
   -> sk : lbuffer uint8 (v crypto_secretkeybytes)
   -> Stack unit
-    (requires fun h -> live h sm /\ live h m /\ live h sk /\ disjoint sm m /\ disjoint sm sk /\ disjoint m sk /\ B.length sm = (v (get h smlen 0)))
-    (ensures fun h0 _ h1 -> live h1 sm /\ live h1 m /\ live h1 sk /\ modifies (loc_buffer sm) h0 h1 /\ 
-                         modifies (loc_buffer smlen) h0 h1)
+    (requires fun h -> live h sm /\ live h m /\ live h sk /\ disjoint sm m /\ disjoint sm sk /\ disjoint m sk /\ smlennat = (v (bget h smlen 0)))
+    (ensures fun h0 _ h1 -> live h1 sm /\ live h1 m /\ live h1 sk /\ modifies2 sm smlen h0 h1)
 
 let crypto_sign #smlennat sm smlen m mlen sk =
     push_frame();
 
-    let c = create #uint8 #(v crypto_c_bytes) crypto_c_bytes (u8 0) in
-    let randomness = create #uint8 #(v crypto_seedbytes) crypto_seedbytes (u8 0) in
+    let c = create crypto_c_bytes (u8 0) in
+    let randomness = create crypto_seedbytes (u8 0) in
     let randomness_input_length:size_t = crypto_randombytes +. crypto_seedbytes +. params_hmbytes in
-    let randomness_input = create #uint8 #(v randomness_input_length) randomness_input_length (u8 0) in
-    let pos_list = create #UI32.t #(v params_h) params_h (UI32.uint_to_t 0) in
-    let sign_list = create #I16.t #(v params_h) params_h (I16.int_to_t 0) in
-    let y:poly = create #_ #(v params_n) params_n (to_elem 0) in	    
-    let y_ntt:poly = create #_ #(v params_n) params_n (to_elem 0) in	    
-    let sc:poly = create #_ #(v params_n) params_n (to_elem 0) in	    
-    let z:poly = create #_ #(v params_n) params_n (to_elem 0) in	    
-    let v_:poly_k = create #_ #(v (params_n *. params_k)) (params_n *. params_k) (to_elem 0) in
-    let ec:poly_k = create #_ #(v (params_n *. params_k)) (params_n *. params_k) (to_elem 0) in
-    let a:poly_k = create #_ #(v (params_n *. params_k)) (params_n *. params_k) (to_elem 0) in
-    let rsp = create #I32.t #1 (size 1) (I32.int_to_t 0) in
-    let nonce = create #I32.t #1 (size 1) (I32.int_to_t 0) in
+    let randomness_input = create randomness_input_length (u8 0) in
+    let pos_list = create params_h (UI32.uint_to_t 0) in
+    let sign_list = create params_h (I16.int_to_t 0) in
+    let y:poly = create params_n (to_elem 0) in
+    let y_ntt:poly = create params_n (to_elem 0) in
+    let sc:poly = create params_n (to_elem 0) in
+    let z:poly = create params_n (to_elem 0) in
+    let v_:poly_k = create (params_n *. params_k) (to_elem 0) in
+    let ec:poly_k = create (params_n *. params_k) (to_elem 0) in
+    let a:poly_k = create (params_n *. params_k) (to_elem 0) in
+    let rsp = create (size 1) (I32.int_to_t 0) in
+    let nonce = create (size 1) (I32.int_to_t 0) in
 
     R.randombytes_ crypto_randombytes (sub randomness_input crypto_randombytes crypto_randombytes);
     update_sub randomness_input (size 0) crypto_seedbytes (sub sk (crypto_secretkeybytes -. crypto_seedbytes) crypto_seedbytes);
@@ -781,66 +789,69 @@ let crypto_sign #smlennat sm smlen m mlen sk =
     do_while
         (fun h _ -> live h c /\ live h randomness /\ live h randomness_input /\
                      live h pos_list /\ live h sign_list /\ live h y /\ live h y_ntt /\ live h sc /\ live h z /\
-		     live h v_ /\ live h ec /\ live h a /\ live h rsp /\ live h nonce /\ live h sm /\ live h m /\ live h sk)
-	(fun _ ->
-	    nonce.(size 0) <- I32.(nonce.(size 0) +^ 1l);
-	    sample_y y randomness (nonce.(size 0));
-	    poly_ntt y_ntt y;
-	    for 0ul params_k
-	        (fun h _ -> live h c /\ live h randomness /\  live h randomness_input /\
+                     live h v_ /\ live h ec /\ live h a /\ live h rsp /\ live h nonce /\ live h sm /\ live h m /\ live h sk)
+        (fun _ ->
+            nonce.(size 0) <- I32.(nonce.(size 0) +^ 1l);
+            sample_y y randomness (nonce.(size 0));
+            poly_ntt y_ntt y;
+            for 0ul params_k
+                (fun h _ -> live h c /\ live h randomness /\  live h randomness_input /\
                      live h pos_list /\ live h sign_list /\ live h y /\ live h y_ntt /\ live h sc /\ live h z /\
-		     live h v_ /\ live h ec /\ live h a /\ live h rsp /\ live h nonce /\ live h sm /\ live h m /\ live h sk)
-		(fun k ->
-		    poly_mul (index_poly v_ k) (index_poly a k) y_ntt
-		);
+                     live h v_ /\ live h ec /\ live h a /\ live h rsp /\ live h nonce /\ live h sm /\ live h m /\ live h sk)
+                (fun k ->
+                    poly_mul (index_poly v_ k) (index_poly a k) y_ntt
+                );
 
-            hash_vm c v_ (sub #_ #_ #(v params_hmbytes) randomness_input (crypto_randombytes +. crypto_seedbytes) params_hmbytes);
-	    encode_c pos_list sign_list c;
-	    sparse_mul8 sc sk pos_list sign_list;
-	    poly_add z y sc;
+            hash_vm c v_ (sub randomness_input (crypto_randombytes +. crypto_seedbytes) params_hmbytes);
+            encode_c pos_list sign_list c;
+            sparse_mul8 sc sk pos_list sign_list;
+            poly_add z y sc;
 
             if test_rejection z
-	    then (false)
-	    else (
-	         push_frame();
-		 let k = create #size_t #1 (size 1) (size 0) in
-		 let break = create #bool #1 (size 1) false in
-	         while
-		 #(fun h -> live h c /\ live h randomness /\  live h randomness_input /\
+            then (false)
+            else (
+                 push_frame();
+                 let k = create (size 1) (size 0) in
+                 let break = create (size 1) false in
+                 while
+                 #(fun h -> live h c /\ live h randomness /\  live h randomness_input /\
                      live h pos_list /\ live h sign_list /\ live h y /\ live h y_ntt /\ live h sc /\ live h z /\
-		     live h v_ /\ live h ec /\ live h a /\ live h rsp /\ live h nonce /\ live h sm /\ live h m /\ live h sk /\ live h k /\ live h break)
-		 #(fun _ h -> live h c /\ live h randomness /\  live h randomness_input /\
+                     live h v_ /\ live h ec /\ live h a /\ live h rsp /\ live h nonce /\ live h sm /\ live h m /\ live h sk /\ live h k /\ live h break)
+                 #(fun _ h -> live h c /\ live h randomness /\  live h randomness_input /\
                      live h pos_list /\ live h sign_list /\ live h y /\ live h y_ntt /\ live h sc /\ live h z /\
-		     live h v_ /\ live h ec /\ live h a /\ live h rsp /\ live h nonce /\ live h sm /\ live h m /\ live h sk /\ live h k /\ live h break)
-                 (fun _ -> let kVal, breakVal = k.(size 0), break.(size 0) in (kVal <. params_k) && (not breakVal))
-                 (fun _ -> 
+                     live h v_ /\ live h ec /\ live h a /\ live h rsp /\ live h nonce /\ live h sm /\ live h m /\ live h sk /\ live h k /\ live h break)
+                 (fun () -> k.(size 0) <. params_k (*&& not break.(size 0)*))
+                 (fun _ ->
                      let kVal:size_t = k.(size 0) in
-		     let sk_offset:size_t = (params_n *. (kVal +. (size 1))) in
-		     let sublen:size_t = crypto_secretkeybytes -. sk_offset in
-		     sparse_mul8 (index_poly ec kVal) (sub #_ #_ #(v sublen) sk sk_offset sublen) pos_list sign_list;
-		     poly_sub (index_poly v_ kVal) (index_poly v_ kVal) (index_poly ec kVal);
-		     rsp.(size 0) <- test_v (index_poly v_ kVal);
-		     if (let rspVal = rsp.(size 0) in not (rspVal = 0l))
-		     then ( break.(size 0) <- true )
-		     else ( k.(size 0) <- UI32.(k.(size 0) +^ 1ul) )
-		 );
-		 pop_frame();
+                     let sk_offset:size_t = (params_n *. (kVal +. (size 1))) in
+                     let sublen:size_t = crypto_secretkeybytes -. sk_offset in
+                     sparse_mul8 (index_poly ec kVal) (sub #_ #_ #(v sublen) sk sk_offset sublen) pos_list sign_list;
+                     poly_sub (index_poly v_ kVal) (index_poly v_ kVal) (index_poly ec kVal);
+                     rsp.(size 0) <- test_v (index_poly v_ kVal);
+                     if (let rspVal = rsp.(size 0) in not (rspVal = 0l))
+                     then ( break.(size 0) <- true )
+                     else ( k.(size 0) <- UI32.(k.(size 0) +^ 1ul) )
+                 );
+                 pop_frame();
 
                  if (let rspVal = rsp.(size 0) in not (rspVal = 0l))
-		 then (false)
-		 else (
-		      for 0ul mlen
-		      (fun h _ -> live h c /\ live h randomness /\  live h randomness_input /\
+                 then (false)
+                 else (
+                      for 0ul mlen
+                      (fun h _ -> live h c /\ live h randomness /\  live h randomness_input /\
                      live h pos_list /\ live h sign_list /\ live h y /\ live h y_ntt /\ live h sc /\ live h z /\
-		     live h v_ /\ live h ec /\ live h a /\ live h rsp /\ live h nonce /\ live h sm /\ live h m /\ live h sk)
-		      (fun i -> upd #_ #smlennat sm (crypto_bytes +. i) (index #_ #mlen m i));
+                     live h v_ /\ live h ec /\ live h a /\ live h rsp /\ live h nonce /\ live h sm /\ live h m /\ live h sk)
+                      (fun i ->
+                        sm.(crypto_bytes +. i) <- B.index m i );
 
                       smlen.(size 0) <- crypto_bytes +. mlen;
 
                       encode_sig sm c z;
 
                       true
-		      )
-		)
-           );          
+                      )
+                )
+           );
     pop_frame()
+
+
